Dafny/examples/Challenge8/Challenge8PropertiesNEW.i.dfy
@@ -4,213 +4,531 @@ include "../../LLVM/types.dfy"
 include "../../LLVM/behaviorLemmas.i.dfy"
 include "../../Libraries/Seqs.s.dfy"
 include "../../Libraries/Seqs.i.dfy"
+include "../../LLVM/memory.i.dfy"
+include "../../LLVM/Operations/binaryOperations.i.dfy"
+include "../../LLVM/ops.dfy"
 
-
-module challenge8Benign{
+module challenge8Properties{
     import opened challenge8CodeNEW
     import opened LLVM_def_NEW
     import opened types
+    import opened memory
     import opened behavior_lemmas
     import opened Collections__Seqs_s
     import opened Collections__Seqs_i
+    import opened binary_operations_i
+    import opened ops
 
-    lemma vulnBehavorsTest(s:state,c:seq<Code>) returns (preB:behavior)
+    lemma vulnRefactor(s:State,c:seq<Code>) returns (preB:Behavior)
         requires ValidState(s);
         requires validStartingState(s);
         requires c == challenge_8_transport_handler_create_conn_vuln_test();
-        // decreases *;
+        ensures ValidBehavior(preB);
+        ensures |preB| == 8;
+        ensures forall i :: i >=0 && i < |preB| - 1 ==> NextStep(preB[i],preB[i+1],Step.stutterStep());
+        ensures preB == [s] + evalCodeSeqFn(c,s);
     {
+        //    [prefixCode(), Block([CNil]),postfixCode()]
+
         reveal_ValidBehavior();
-        //    [ Block([CNil]), Block([CNil]), Block([CNil])]
-        var b:behavior := evalCodeSeqFn(c,s);
-        assert ValidBehaviorV2([s] + b);
-        assert |b| >= 0;
-        assert c == [ Block([CNil]), Block([CNil]), Block([CNil])];
-
-        var step,remainder,subB := unwrapCodeWitness(b,c,s);
-        assert step == evalCodeFn(Block([CNil]),s);
-        assert remainder == [Block([CNil]), Block([CNil])];
-        // lets dive into the block
-            var subStep,subRemainder,subSubB := unwrapCodeWitness(step,[CNil],s);
-            assert subStep == [s];
-            assert subRemainder == [];
-            assert subSubB == [s];
-            // unwrapped entire subBlock
-        assert step == subStep+subSubB;
-        assert b[..|step|] == step;
-
-        var s' := last(step);
-        step,remainder,subB := unwrapCodeWitness(subB,remainder,s');
-        assert step == evalCodeFn(Block([CNil]),s');
-        assert remainder == [ Block([CNil])];
-            // lets dive into the block
-            subStep,subRemainder,subSubB := unwrapCodeWitness(step,[CNil],s');
-            assert subStep == [s'];
-            assert subRemainder == [];
-            assert subSubB == [s'];
-
-         assert step == subStep+subSubB;
-        assert couldBeSubSeq(b,step);
-
-        s' := last(step);
-        step,remainder,subB := unwrapCodeWitness(subB,remainder,s');
-        assert step == evalCodeFn(Block([CNil]),s');
-        assert remainder == [];
-
-        assert subB == [s'];
+        var b:Behavior := [s] + evalCodeSeqFn(c,s);
+        assert |b| == 8;
         assert ValidBehavior(b);
-        assert NextStep(b[0],b[1],Step.stutterStep());
-        assert StateNext(b[0],b[1]);
-        assert NextStep(b[1],b[2],Step.stutterStep());
-        assert StateNext(b[1],b[2]);
-        assert |b| == 7;
+        forall i | i >=0 && i < |b| - 1
+            ensures  NextStep(b[i],b[i+1],Step.stutterStep());
+        {
+            // assert NextStep(b[i],b[i+1],Step.stutterStep());
+        }
+
+        var prefixB :=  [s] + evalCodeFn(prefixCode(),s);
+        assert |prefixB| == 3;
+        assert prefixB == b[..3];
+
+        var midB :=  evalCodeFn(Block([CNil]),last(prefixB));
+        assert |midB| == 2;
+        assert midB == b[3..5];
+
+        var postfixB :=  evalCodeFn(postfixCode(),last(midB));
+        assert |postfixB| == 2;
+
+        assert b == prefixB + midB + postfixB + [last(postfixB)];
+
         preB := b;
+
     }
 
-lemma patchBehavorsTest(s:state,c:seq<Code>) returns (postB:behavior)
+    lemma patchRefactor(s:State,c:seq<Code>,size:Operand) returns (postB:Behavior)
         requires ValidState(s);
         requires validStartingState(s);
-        requires c == challenge_8_transport_handler_create_conn_patch();
-        // decreases *;
+        requires size.D?;
+        requires size.d.Int?;
+        requires size.d.itype == IntType(4,false);
+        requires ValidOperand(s,size)
+        requires c == challenge_8_transport_handler_create_conn_patch(size);
+        requires validConfig(s);
+
+        ensures postB ==  [s] + evalCodeSeqFn(c,s);
     {
         reveal_ValidBehavior();
-        //    [ Block([CNil]), Block([CNil]), Block([CNil])]
-        var b:behavior := evalCodeSeqFn(c,s);
-        assert ValidBehaviorV2([s] + b);
-        assert |b| >= 0;
+        var config := allVariablesConfig();    
+        postB := [s] + evalCodeSeqFn(c,s);
+        // assert postB == [s] + evalCodeSeqFn(c,s)
+        var prefixB :=  [s] + evalCodeFn(prefixCode(),s);
+        var mid := evalCodeFn(patch_block(size),last(prefixB));
+        var post := evalCodeFn(postfixCode(),last(mid));
+        assert all_but_last(prefixB) == postB[..2];
+        // assert all_but_last(mid) ==  postB[2..2+|mid|];
+        // assert postB == all_but_last(prefixB) +  all_but_last(mid) + post;
+        // assert |prefixB| == 3;
+        // var vulnB := vulnRefactor(s,challenge_8_transport_handler_create_conn_vuln_test());
+        // var vb:Behavior := [s] + evalCodeSeqFn(challenge_8_transport_handler_create_conn_vuln_test(),s);
+        // assert prefixB == vulnB[..3];
+        // assert prefixB == postB[..3];
         
-        var step,remainder,subB := unwrapCodeWitness(b,c,s);
-        assert step == evalCodeFn(Block([CNil]),s);
-        // assert remainder == [patch_block,postfixCode()];
-        // lets dive into the block
-            var subStep,subRemainder,subSubB := unwrapCodeWitness(step,[CNil],s);
-            assert subStep == [s];
-            assert subRemainder == [];
-            assert subSubB == [s];
-            // unwrapped entire subBlock
-        assert step == subStep+subSubB;
-        assert b[..|step|] == step;
+        // assert s == postB[1] == postB[2] == postB[0];
+        assert NextStep(postB[0],postB[1],Step.stutterStep());
+        assert NextStep(postB[1],postB[2],Step.stutterStep());
 
-        var s' := last(step);
-        var mainBlock := remainder;
-        // assert re
-        step,remainder,subB := unwrapCodeWitness(subB,remainder,s');
-        assert remainder == [ Block([CNil])];
-         // lets dive into the block
-            assert step == evalCodeFn(first(mainBlock),s');
-            assert first(mainBlock).Block?;
-            assert step == evalCodeSeqFn(first(mainBlock).block,s');
+        // assert (config.ops["var_div"].LV? || config.ops["var_div"].GV?)  
+        //         && ValidOperand(postB[2],config.ops["var_div"]) && ValidOperand(s,size) 
+        //         && ValidOperand(postB[2],D(Int(7,IntType(4,false))));
+        // assert isInt(OperandContents(postB[2],size)); 
+        // assert typesMatch(OperandContents(postB[2],size),OperandContents(postB[2],D(Int(7,IntType(4,false)))));
+        assert ValidState(postB[2]);
+        assert ValidInstruction(postB[2], (SDIV(config.ops["var_div"],size,D(Int(7,IntType(4,false))))));
+        var s'' := stateUpdateVar(postB[2],config.ops["var_div"],evalSDIV(OperandContents(postB[2],size),OperandContents(postB[2],D(Int(7,IntType(4,false))))));
+        s'' :=  incPC(s'');
+        assert ValidData(s'',evalSDIV(OperandContents(postB[2],size),OperandContents(postB[2],D(Int(7,IntType(4,false))))));
+        assert s''.ok;
+        assert patch_block(size).block[0] == Ins(SDIV(config.ops["var_div"],size,D(Int(7,IntType(4,false)))));
+        assert ValidState(s'');
+        assert  config.ops["var_div"].LV?;
+        assert s''.pc == postB[2].pc +1;
+        assert s'' == postB[2].(lvs := postB[2].lvs[config.ops["var_div"].l := evalSDIV(OperandContents(postB[2],size),OperandContents(postB[2],D(Int(7,IntType(4,false)))))],o := Nil,pc := postB[2].pc +1); 
+        // assert evalUpdate(postB[2], config.ops["var_div"], evalSDIV(OperandContents(postB[2],size),OperandContents(postB[2],D(Int(7,IntType(4,false))))),s'');
+        // assert postB[3] == evalInsRe((SDIV(config.ops["var_div"],size,D(Int(7,IntType(4,false))))),post[2]);
+        assert validEvalIns((SDIV(config.ops["var_div"],size,D(Int(7,IntType(4,false))))),postB[2],s'');
 
-            // assert step == evalCodeSeqFn(first(mainBlock),s');
-            subStep,subRemainder,subSubB := unwrapCodeWitness(step,first(mainBlock).block,s');
-            assert |subStep| == 1;
-            assert s'.ok;
-            assert first(mainBlock).block[0].Ins?;
-            assert first(mainBlock).block[0].ins.SDIV?;
-            assert ValidOperand(s',first(mainBlock).block[0].ins.dst);
-            var testIns := first(mainBlock).block[0].ins;
-                
-            assert ValidInstruction(s', first(mainBlock).block[0].ins);
-            assert NextStep(s',subStep[0],Step.evalInsStep(first(mainBlock).block[0].ins));
-            // assert subRemainder == [];
-            assert b[1] == s';
-            assert b[2] == subStep[0];  
-            s' := subStep[0];
-            var nextIns := subRemainder;
-            subStep,subRemainder,subSubB := unwrapCodeWitness(subSubB,subRemainder,s');
-            assert |subStep| == 1;
-            assert NextStep(s',subStep[0],Step.evalInsStep(first(nextIns).ins));
-            assert b[3] == subStep[0];
-            assert ValidInstruction(s', first(nextIns).ins);
-
-            s' := subStep[0];
-            nextIns := subRemainder;
-            assert first(subRemainder).IfElse?;
-            assert validIfCond(s',first(subRemainder).ifCond);
-                //unwrap branch
-            assert |subRemainder| > 0;
-            subStep,subRemainder,subSubB := unwrapCodeWitness(subSubB,subRemainder,s');
-             
-                if dataToBool(OperandContents(s',first(nextIns).ifCond)){
-                    assert subStep == evalCodeFn(first(nextIns).ifTrue,s');
-                    // new block that needs unwrapping 
-                    patchBehavorsTestsubBlock(subStep,first(nextIns).ifTrue,s');
-                    // var if_true_block := first(nextIns).ifTrue;
-                    // var step_if_then19,remainder_if_then19,subB_if_then19 := unwrapCodeWitness(subStep,if_true_block.block,s');
-                    // assert |step_if_then19| == 1;
-                    // assert first(if_true_block.block).Ins?;
-                    // assert first(if_true_block.block).ins.CALL?;
-                    // assert NextStep(s',step_if_then19[0],Step.evalInsStep(first(if_true_block.block).ins));
-
-                    // var if_true_next := first(remainder_if_then19);
-                    // s' := first(step_if_then19); 
-                    // step_if_then19,remainder_if_then19,subB_if_then19 := unwrapCodeWitness(subB_if_then19,remainder_if_then19,s');
-                    // assert |step_if_then19| == 1;
-                    // assert NextStep(s',step_if_then19[0],Step.evalInsStep((if_true_next).ins));
-                    // assert |remainder_if_then19| == 1;
+        // assert ValidState(x);
+        assert NextStep(postB[2],postB[3],evalInsStep((SDIV(config.ops["var_div"],size,D(Int(7,IntType(4,false)))))));
+        // assert ValidState(postB[3]);
+        // assert NextStep(postB[3],postB[4],evalInsStep((ICMP(config.ops["var_cmp17"],sgt,4,config.ops["var_num_packets"],config.ops["var_div"]))));
+        // if dataToBool(OperandContents(postB[4],config.ops["var_cmp17"])){
+        // //     assert NextStep(postB[4],postB[5],evalInsStep((CALL(D(Void),delete_connection()))));
+        // }else{
+        // //     assert NextStep(postB[4],postB[5],Step.stutterStep());
+        // }
+        // assert NextStep(postB[4],postB[5],evalInsStep((ICMP(config.ops["var_cmp17"],sgt,4,config.ops["var_num_packets"],config.ops["var_div"]))));
 
 
-                }else{
-                    assert subStep == evalCodeFn(first(nextIns).ifFalse,s');
-                    assert subRemainder == [];
-                    assert subSubB == [s']; 
-                    assert b[4] == subStep[0]; 
-                    assert b[5] == subStep[0];
-                    assert |b| == 10;
-                }
-        
-        s' := last(step);
-        step,remainder,subB := unwrapCodeWitness(subB,remainder,s');
-        assert step == evalCodeFn(Block([CNil]),s');
-        assert remainder == [];
-
-        assert subB == [s'];
-
-
-            // assert subSubB == [s];
-
-
+        // assert vb
     }
 
-    lemma {:opaque} patchBehavorsTestsubBlock(b:behavior,c:Code,s:state)
-        requires c == if_then19();
-        requires ValidState(s);
-        requires validConfig(s,allVariablesConfig());
-        requires b == evalCodeSeqFn(c.block,s);
-        ensures  first(c.block).Ins?;
-        ensures first(c.block).ins.CALL?;
-        
-        
+    lemma behaviorIsSumOfParts(s:State,cseq:seq<Code>,b:Behavior)
+        requires b == [s] + evalCodeSeqFn(cseq,s)
+        requires |cseq| > 1;
     {
-        var behavior := evalCodeSeqFn(c.block,s);
-        var initalCode := c.block;
-        var step,remainder,subB := unwrapCodeWitness(b,c.block,s);
-        assert |step| == 1;
-        assert first(initalCode).Ins?;
-        assert first(initalCode).ins.CALL?;
-        assert StateNext(s,step[0]);
-        // assert step == [evalInsRe(first(initalCode).ins,s)];
-        // assert s.ok;
-        assert NextStep(s,step[0],Step.evalInsStep(first(initalCode).ins));
-        initalCode := remainder;
-        var s' := step[0];
-        assert ValidState(s');
-        step,remainder,subB := unwrapCodeWitness(subB,remainder,last(step));
-        assert |step| == 1;
-        assert first(initalCode).Ins?;
-        assert first(initalCode).ins.STORE?; 
-        // assert ensures first(c.block).ins.STORE?;
-        // assert s'.ok;
-        // assert ValidOperand(s',first(initalCode).ins.valueToStore);
-        // assert ValidOperand(s',first(initalCode).ins.ptr);
-        // assert ValidInstruction(s',first(initalCode).ins);
-        // assert NextStep(s',step[0],Step.evalInsStep(first(initalCode).ins));
+        var smalB := b;
+        assert smalB[..1] == [s];
+        smalB := smalB[1..];
+        // var index := 1;
+        var i := 0;
+        var subB := evalCodeFn(cseq[i],s);
+        assert smalB[..|subB|] == subB;
+        
+        smalB := smalB[|subB|..];
 
-        // assert false;
+        assert evalCodeSeqFn(cseq,s) == evalCodeFn(first(cseq),s) + evalCodeSeqFn(all_but_first(cseq),last(evalCodeFn(first(cseq),s)));
+        assert subB ==  evalCodeFn(first(cseq),s);
+        // assert evalCodeSeqFn(all_but_first(cseq),last(evalCodeFn(first(cseq),s))) == evalCodeFn(first(all_but_first(cseq)),last(evalCodeFn(first(cseq),s)))
+        // index := 1+|subB|;
+        // i := i +1;
+        // subB := evalCodeFn(cseq[i],last(subB));
+        // assert b[..|subB|] == subB;
+        // while i < |cseq|
+        // {
+        //     var subB := evalCodeFn(cseq[i],b[index-1]);
+        //     assert b[index..index+|subB|] == subB;
+        //     index := index+|subB|;
+        //     i := i +1;
+        // }
+    //    forall i | i >= 0 && i < |cseq|
+    //    {
+    //      var subB := evalCodeFn(prefixCode(),b[index-1]);
+    //      assert b[index..index+|subB|] == subB;
+    //      index := index+|subB|;
+    //    }
+    }
+
+    lemma fullPatch(s:State,size:Operand)returns (b:Behavior)
+        requires ValidState(s);
+        requires validStartingState(s);
+        requires size.D?;
+        requires size.d.Int?;
+        requires size.d.itype == IntType(4,false);
+        requires ValidOperand(s,size)
+        requires validConfig(s);
+        ensures b ==  [s] + evalCodeSeqFn(challenge_8_transport_handler_create_conn_patch(size),s);
+    {
+        var config := allVariablesConfig();    
+        b := [s] + evalCodeSeqFn(challenge_8_transport_handler_create_conn_patch(size),s);   
+        var prefixB :=  [s] + evalCodeFn(prefixCode(),s);
+        var mid := evalCodeFn(patch_block(size),last(prefixB));
+        // var post := evalCodeFn(postfixCode(),last(mid));
+
+        assert NextStep(b[0],b[1],Step.stutterStep());
+        assert NextStep(b[1],b[2],Step.stutterStep());
+        assert last(prefixB) == b[2];
+        // assert b == prefixB + mid + post + [last(post)];
+        assert b == prefixB + mid  + [last(mid)];
+
+        // var x := patchBlock(b[2],size);
+        // assert mid == all_but_first(x);
+
+        // assert |post| == 2;
+        // assert forall i :: i>= |b|-3 && i < |b| ==> b[i] == last(mid);
+        // assert NextStep(b[3],b[4],evalInsStep((ICMP(config.ops["var_cmp17"],sgt,4,config.ops["var_num_packets"],config.ops["var_div"]))));
+        // assert size.d.val/7 < (OperandContents(b[4],config.ops["var_num_packets"]).val) ==> !dataToBool(OperandContents(b[4],config.ops["var_cmp17"]));
+
+    }
+
+    predicate miniSpec(s:State,b:Behavior,size:Operand)
+        requires size.D?;
+        requires size.d.Int?;
+        requires size.d.itype == IntType(4,false);
+    {
+       assert forall s :: |evalCodeFn(postfixCodeSimple(),s)| == 4;
+        var config := allVariablesConfig();
+
+       && b == [s] + evalCodeFn(patch_block(size),s)
+       && |b| >= 8
+       && b[|b|-5..] == evalCodeFn(postfixCodeSimple(),b[|b|-6]) + [last(b)]
+       && FromTwosComp(UInt32(size.d.val/Int(7,IntType(4,false)).val % 0x8000_0000)).val < (OperandContents(s,config.ops["var_num_packets"]).val)
     }
 
 
-    // lemma patchBehaviors(s:state,c:codeRe) returns (postB:behavior)
+    lemma patchBlock(s:State,size:Operand) returns (b:Behavior)
+        requires ValidState(s);
+        requires validStartingState(s);
+        requires size.D?;
+        requires size.d.Int?;
+        requires size.d.itype == IntType(4,false);
+        requires ValidOperand(s,size)
+        requires validConfig(s);
+        ensures b ==  [s] + evalCodeFn(patch_block(size),s);
+        ensures |b| >= 8;
+        ensures !miniSpec(s,b,size);
+        // ensures ValidBehavior(b);
+    {
+        var config := allVariablesConfig();
+        b := [s] + evalCodeFn(patch_block(size),s);
+
+        assert NextStep(b[0],b[1],evalInsStep((SDIV(config.ops["var_div"],size,D(Int(7,IntType(4,false)))))));
+        // assert ValidState(b[1]);
+        assert NextStep(b[1],b[2],evalInsStep((ICMP(config.ops["var_cmp17"],sgt,4,config.ops["var_num_packets"],config.ops["var_div"]))));
+        if dataToBool(OperandContents(b[2],config.ops["var_cmp17"])){
+            // assert evalCodeFn(c.ifTrue,s);
+            assert patch_block(size).block[2].IfElse?;
+            var ifElseB := evalCodeFn(patch_block(size).block[2].ifTrue,b[2]);
+            assert b == [s] + [b[1]] + [b[2]] + ifElseB + [last(ifElseB)];
+            var ifThen19:Behavior := ifThen19(b[2]);
+            assert [b[2]] + evalCodeFn(patch_block(size).block[2].ifTrue,b[2]) == ifThen19; 
+            // assert b == [s] + [b[1]] + ifThen19 + [last(ifThen19)];
+
+                        // assert |ifElseB| == |ifThen19|;
+
+            assert b[2..2+|ifThen19|] == ifThen19;
+            assert b[2..] == ifThen19 + [last(ifThen19)];
+            assert NextStep(b[2],b[3],evalInsStep((CALL(D(Void),delete_connection()))));
+            assert NextStep(b[3],b[4],evalInsStep((STORE(D(Int(0,IntType(1,false))),allVariablesConfig().ops["var_retval"]))));
+            assert NextStep(b[4],b[5],evalInsStep((LOAD(allVariablesConfig().ops["var_26"],1,allVariablesConfig().ops["var_retval"]))));
+            assert NextStep(b[5],b[6],evalInsStep((RET(allVariablesConfig().ops["var_26"]))));
+            assert NextStep(b[6],b[7],Step.stutterStep());
+            assert NextStep(b[7],b[8],Step.stutterStep());
+
+            assert NextStep(b[8],b[9],Step.stutterStep());
+            // assert OperandContents(b[9],allVariablesConfig().ops["var_26"]).val == 0;
+            assert |b| == 10;
+            assert !miniSpec(s,b,size);
+        }else{
+            assert NextStep(b[2],b[3],evalInsStep((STORE(D(Int(1,IntType(1,false))),allVariablesConfig().ops["var_retval"]))));
+            assert NextStep(b[3],b[4],evalInsStep((LOAD(allVariablesConfig().ops["var_26"],1,allVariablesConfig().ops["var_retval"]))));
+            assert NextStep(b[4],b[5],evalInsStep((RET(allVariablesConfig().ops["var_26"]))));
+           
+            assert NextStep(b[5],b[6],Step.stutterStep());
+            assert NextStep(b[6],b[7],Step.stutterStep());
+            // assert NextStep(b[4],b[5],Step.stutterStep());
+            assert |b| == 8;
+            assert !miniSpec(s,b,size);
+        }
+        // assert (OperandContents(b[2],config.ops["var_num_packets"]).val) > (OperandContents(b[2],config.ops["var_div"]).val) ==> dataToBool(OperandContents(b[2],config.ops["var_cmp17"]));
+        // assert OperandContents(b[1],config.ops["var_div"]).val == FromTwosComp(UInt32(size.d.val/Int(7,IntType(4,false)).val % 0x8000_0000)).val;
+        // assert OperandContents(b[1],config.ops["var_div"]).val > (OperandContents(b[1],config.ops["var_num_packets"]).val) ==> OperandContents(b[2],config.ops["var_cmp17"]).val == 0;
+        // assert OperandContents(b[1],config.ops["var_div"]).val > (OperandContents(b[1],config.ops["var_num_packets"]).val) ==>!dataToBool(OperandContents(b[2],config.ops["var_cmp17"]));
+        // assert FromTwosComp(UInt32(size.d.val/Int(7,IntType(4,false)).val % 0x8000_0000)).val > (OperandContents(b[1],config.ops["var_num_packets"]).val) ==> |b| == 8;
+        // assert FromTwosComp(UInt32(size.d.val/Int(7,IntType(4,false)).val % 0x8000_0000)).val < (OperandContents(b[2],config.ops["var_num_packets"]).val) ==> !dataToBool(OperandContents(b[2],config.ops["var_cmp17"]));
+    }
+
+    lemma returnBlock(s:State) returns (b:Behavior)
+        requires ValidState(s);
+        requires validIntState(s);
+        requires validConfig(s);
+        ensures b == [s] + evalCodeFn(return_(),s);
+        ensures |b| == 4;
+        ensures NextStep(b[0],b[1],evalInsStep((LOAD(allVariablesConfig().ops["var_26"],1,allVariablesConfig().ops["var_retval"]))));
+        ensures NextStep(b[1],b[2],evalInsStep((RET(allVariablesConfig().ops["var_26"]))));
+        ensures NextStep(b[2],b[3],Step.stutterStep());
+    {
+    var config := allVariablesConfig();
+
+    b := [s] + evalCodeFn(return_(),s);
+    assert StateNext(b[0],b[1]);
+    assert ValidState(b[1]);
+    assert ValidState(b[2]);
+    assert ValidState(b[3]);
+    assert |b| == 4;
+    assert NextStep(b[0],b[1],evalInsStep((LOAD(config.ops["var_26"],1,config.ops["var_retval"]))));
+    assert NextStep(b[1],b[2],evalInsStep((RET(config.ops["var_26"]))));
+    assert NextStep(b[2],b[3],Step.stutterStep());
+
+}
+
+lemma ifThen19(s:State) returns (b:Behavior)
+    requires ValidState(s);
+    requires validIntState(s);
+    requires validConfig(s);
+    ensures b == [s] + evalCodeFn(if_then19(),s);
+    ensures |b| == 7;
+    ensures NextStep(b[0],b[1],evalInsStep((CALL(D(Void),delete_connection()))));
+    ensures NextStep(b[1],b[2],evalInsStep((STORE(D(Int(0,IntType(1,false))),allVariablesConfig().ops["var_retval"]))));
+    ensures NextStep(b[2],b[3],evalInsStep((LOAD(allVariablesConfig().ops["var_26"],1,allVariablesConfig().ops["var_retval"]))));
+    ensures NextStep(b[3],b[4],evalInsStep((RET(allVariablesConfig().ops["var_26"]))));
+    ensures NextStep(b[4],b[5],Step.stutterStep());
+    ensures NextStep(b[5],b[6],Step.stutterStep());
+
+{
+    var config := allVariablesConfig();
+
+    b := [s] + evalCodeFn(if_then19(),s);
+    assert |b| == 7;
+    assert NextStep(b[0],b[1],evalInsStep((CALL(D(Void),delete_connection()))));
+    // assert  ValidState(b[1]);
+    // assert ValidInstruction(b[1], (CALL(D(Void),delete_connection())));
+    // assert if_then19().block[1].Ins?;
+    // assert MemValid(b[2].m);
+    // assert if_then19().block[1].ins == (STORE(D(Int(0,IntType(1,false))),config.ops["var_retval"]));
+    // assert NextStep(b[1],b[2],Step.stutterStep());
+    assert NextStep(b[1],b[2],evalInsStep((STORE(D(Int(0,IntType(1,false))),config.ops["var_retval"]))));
+    // assert if_then19().block[2].Block?;
+    // assert if_then19().block[2] == return_();
+    // assert [b[0],b[1],b[2]] == b[..3];
+    // assert NextStep(b[2],b[3],evalInsStep((LOAD(config.ops["var_26"],1,config.ops["var_retval"]))));
+    // assert NextStep(b[3],b[4],evalInsStep((RET(config.ops["var_26"]))));
+    // assert NextStep(b[4],b[5],Step.stutterStep());
+    // assert NextStep(b[5],b[6],Step.stutterStep());
+    var rB := returnBlock(b[2]);
+    assert NextStep(b[5],b[6],Step.stutterStep());
+}
+
+// lemma
+
+
+//     lemma vulnBehavorsTest(s:State,c:seq<Code>) returns (preB:Behavior)
+//         requires ValidState(s);
+//         requires validStartingState(s);
+//         requires c == challenge_8_transport_handler_create_conn_vuln_test();
+//         // decreases *;
+//     {
+//         reveal_ValidBehavior();
+//         //    [ Block([CNil]), Block([CNil]), Block([CNil])]
+//         var b:Behavior := evalCodeSeqFn(c,s);
+//         assert ValidSimpleBehavior([s] + b);
+//         assert |b| >= 0;
+//         assert c == [ Block([CNil]), Block([CNil]), Block([CNil])];
+
+//         var step,remainder,subB := unwrapCodeWitness(b,c,s);
+//         assert step == evalCodeFn(Block([CNil]),s);
+//         assert remainder == [Block([CNil]), Block([CNil])];
+//         // lets dive into the block
+//             var subStep,subRemainder,subSubB := unwrapCodeWitness(step,[CNil],s);
+//             assert subStep == [s];
+//             assert subRemainder == [];
+//             assert subSubB == [s];
+//             // unwrapped entire subBlock
+//         assert step == subStep+subSubB;
+//         assert b[..|step|] == step;
+
+//         var s' := last(step);
+//         step,remainder,subB := unwrapCodeWitness(subB,remainder,s');
+//         assert step == evalCodeFn(Block([CNil]),s');
+//         assert remainder == [ Block([CNil])];
+//             // lets dive into the block
+//             subStep,subRemainder,subSubB := unwrapCodeWitness(step,[CNil],s');
+//             assert subStep == [s'];
+//             assert subRemainder == [];
+//             assert subSubB == [s'];
+
+//          assert step == subStep+subSubB;
+//         assert couldBeSubSeq(b,step);
+
+//         s' := last(step);
+//         step,remainder,subB := unwrapCodeWitness(subB,remainder,s');
+//         assert step == evalCodeFn(Block([CNil]),s');
+//         assert remainder == [];
+
+//         assert subB == [s'];
+//         assert ValidBehavior(b);
+//         assert NextStep(b[0],b[1],Step.stutterStep());
+//         assert StateNext(b[0],b[1]);
+//         assert NextStep(b[1],b[2],Step.stutterStep());
+//         assert StateNext(b[1],b[2]);
+//         assert |b| == 7;
+//         preB := b;
+//     }
+
+
+
+// lemma patchBehavorsTest(s:State,c:seq<Code>) returns (postB:Behavior)
+//         requires ValidState(s);
+//         requires validStartingState(s);
+//         requires c == challenge_8_transport_handler_create_conn_patch();
+//         // decreases *;
+//     {
+//         reveal_ValidBehavior();
+//         //    [ Block([CNil]), Block([CNil]), Block([CNil])]
+//         // var b:Behavior := evalCodeSeqFn(c,s);
+//         // assert ValidSimpleBehavior([s] + b);
+//         // assert |b| >= 0;
+        
+//         // var step,remainder,subB := unwrapCodeWitness(b,c,s);
+//         // assert step == evalCodeFn(Block([CNil]),s);
+//         // // assert remainder == [patch_block,postfixCode()];
+//         // // lets dive into the block
+//         //     var subStep,subRemainder,subSubB := unwrapCodeWitness(step,[CNil],s);
+//         //     assert subStep == [s];
+//         //     assert subRemainder == [];
+//         //     assert subSubB == [s];
+//         //     // unwrapped entire subBlock
+//         // assert step == subStep+subSubB;
+//         // assert b[..|step|] == step;
+
+//         // var s' := last(step);
+//         // var mainBlock := remainder;
+//         // // assert re
+//         // step,remainder,subB := unwrapCodeWitness(subB,remainder,s');
+//         // assert remainder == [ Block([CNil])];
+//         //  // lets dive into the block
+//         //     assert step == evalCodeFn(first(mainBlock),s');
+//         //     assert first(mainBlock).Block?;
+//         //     assert step == evalCodeSeqFn(first(mainBlock).block,s');
+
+//         //     // assert step == evalCodeSeqFn(first(mainBlock),s');
+//         //     subStep,subRemainder,subSubB := unwrapCodeWitness(step,first(mainBlock).block,s');
+//         //     assert |subStep| == 1;
+//         //     assert s'.ok;
+//         //     assert first(mainBlock).block[0].Ins?;
+//         //     assert first(mainBlock).block[0].ins.SDIV?;
+//         //     assert ValidOperand(s',first(mainBlock).block[0].ins.dst);
+//         //     var testIns := first(mainBlock).block[0].ins;
+                
+//         //     assert ValidInstruction(s', first(mainBlock).block[0].ins);
+//         //     assert NextStep(s',subStep[0],Step.evalInsStep(first(mainBlock).block[0].ins));
+//         //     // assert subRemainder == [];
+//         //     assert b[1] == s';
+//         //     assert b[2] == subStep[0];  
+//         //     s' := subStep[0];
+//         //     var nextIns := subRemainder;
+//         //     subStep,subRemainder,subSubB := unwrapCodeWitness(subSubB,subRemainder,s');
+//         //     assert |subStep| == 1;
+//         //     assert NextStep(s',subStep[0],Step.evalInsStep(first(nextIns).ins));
+//         //     assert b[3] == subStep[0];
+//         //     assert ValidInstruction(s', first(nextIns).ins);
+
+//         //     s' := subStep[0];
+//         //     nextIns := subRemainder;
+//         //     assert first(subRemainder).IfElse?;
+//         //     assert validIfCond(s',first(subRemainder).ifCond);
+//         //         //unwrap branch
+//         //     assert |subRemainder| > 0;
+//         //     subStep,subRemainder,subSubB := unwrapCodeWitness(subSubB,subRemainder,s');
+             
+//         //         if dataToBool(OperandContents(s',first(nextIns).ifCond)){
+//         //             assert subStep == evalCodeFn(first(nextIns).ifTrue,s');
+//         //             // new block that needs unwrapping 
+//         //             patchBehavorsTestsubBlock(subStep,first(nextIns).ifTrue,s');
+//         //             // var if_true_block := first(nextIns).ifTrue;
+//         //             // var step_if_then19,remainder_if_then19,subB_if_then19 := unwrapCodeWitness(subStep,if_true_block.block,s');
+//         //             // assert |step_if_then19| == 1;
+//         //             // assert first(if_true_block.block).Ins?;
+//         //             // assert first(if_true_block.block).ins.CALL?;
+//         //             // assert NextStep(s',step_if_then19[0],Step.evalInsStep(first(if_true_block.block).ins));
+
+//         //             // var if_true_next := first(remainder_if_then19);
+//         //             // s' := first(step_if_then19); 
+//         //             // step_if_then19,remainder_if_then19,subB_if_then19 := unwrapCodeWitness(subB_if_then19,remainder_if_then19,s');
+//         //             // assert |step_if_then19| == 1;
+//         //             // assert NextStep(s',step_if_then19[0],Step.evalInsStep((if_true_next).ins));
+//         //             // assert |remainder_if_then19| == 1;
+
+
+//         //         }else{
+//         //             assert subStep == evalCodeFn(first(nextIns).ifFalse,s');
+//         //             assert subRemainder == [];
+//         //             assert subSubB == [s']; 
+//         //             assert b[4] == subStep[0]; 
+//         //             assert b[5] == subStep[0];
+//         //             assert |b| == 10;
+//         //         }
+        
+//         // s' := last(step);
+//         // step,remainder,subB := unwrapCodeWitness(subB,remainder,s');
+//         // assert step == evalCodeFn(Block([CNil]),s');
+//         // assert remainder == [];
+
+//         // assert subB == [s'];
+
+
+//     }
+
+//     lemma {:opaque} patchBehavorsTestsubBlock(b:Behavior,c:Code,s:State)
+//         requires c == if_then19();
+//         requires ValidState(s);
+//         requires validConfig(s,allVariablesConfig());
+//         requires b == evalCodeSeqFn(c.block,s);
+//         ensures  first(c.block).Ins?;
+//         ensures first(c.block).ins.CALL?;
+        
+        
+//     {
+//         var Behavior := evalCodeSeqFn(c.block,s);
+//         var initalCode := c.block;
+//         var step,remainder,subB := unwrapCodeWitness(b,c.block,s);
+//         assert |step| == 1;
+//         assert first(initalCode).Ins?;
+//         assert first(initalCode).ins.CALL?;
+//         assert StateNext(s,step[0]);
+//         // assert step == [evalInsRe(first(initalCode).ins,s)];
+//         // assert s.ok;
+//         assert NextStep(s,step[0],Step.evalInsStep(first(initalCode).ins));
+//         initalCode := remainder;
+//         var s' := step[0];
+//         assert ValidState(s');
+//         step,remainder,subB := unwrapCodeWitness(subB,remainder,last(step));
+//         assert |step| == 1;
+//         assert first(initalCode).Ins?;
+//         assert first(initalCode).ins.STORE?; 
+//         // assert ensures first(c.block).ins.STORE?;
+//         // assert s'.ok;
+//         // assert ValidOperand(s',first(initalCode).ins.valueToStore);
+//         // assert ValidOperand(s',first(initalCode).ins.ptr);
+//         // assert ValidInstruction(s',first(initalCode).ins);
+//         // assert NextStep(s',step[0],Step.evalInsStep(first(initalCode).ins));
+
+//         // assert false;
+//     }
+
+
+    // lemma patchBehaviors(s:State,c:codeRe) returns (postB:Behavior)
     //     requires ValidState(s);
     //     requires validStartingState(s);
     //     requires c == challenge_8_transport_handler_create_conn_patch();
@@ -272,7 +590,7 @@ lemma patchBehavorsTest(s:state,c:seq<Code>) returns (postB:behavior)
     // }
 
     //     // benignPatch: "The patch does not add any NEW behaviors"
-    // predicate benignPatch(pre:set<behavior>,post:set<behavior>)
+    // predicate benignPatch(pre:set<Behavior>,post:set<Behavior>)
     // {
     //     var preOutput := allBehaviorOutputSet(pre);
     //     var postOutput := allBehaviorOutputSet(post);
@@ -296,7 +614,7 @@ lemma patchBehavorsTest(s:state,c:seq<Code>) returns (postB:behavior)
     // }
 
     // // Proof
-    // function vulnified(s:state) : (s_vuln:state)
+    // function vulnified(s:State) : (s_vuln:State)
     // {
     //     // assume exists vuln :: BehaviorEvalsCode(challenge_8_transport_handler_create_conn_vuln(),vuln) && |vuln| > 0;
     //     // var vuln :| BehaviorEvalsCode(challenge_8_transport_handler_create_conn_vuln(),vuln);
@@ -306,12 +624,12 @@ lemma patchBehavorsTest(s:state,c:seq<Code>) returns (postB:behavior)
     //     s
     // }
 
-    // function patchified(s:state) : state
+    // function patchified(s:State) : State
     // {
     //     s
     // }
 
-    // function mapPatchedToVuln(patchedBehavior:behavior) : (mappedBehavior:behavior)
+    // function mapPatchedToVuln(patchedBehavior:Behavior) : (mappedBehavior:Behavior)
     //     // requires BehaviorEvalsCode(challenge_8_transport_handler_create_conn_patch(),patchedBehavior)
     //     ensures |patchedBehavior| == |mappedBehavior|
     //     ensures forall i :: (i >= 0 && i < |patchedBehavior|) ==> mappedBehavior[i] == vulnified(patchedBehavior[i])
@@ -328,7 +646,7 @@ lemma patchBehavorsTest(s:state,c:seq<Code>) returns (postB:behavior)
         
     // }
 
-    //  function mapVulnToPatched(vulnBehaviors:behavior) : (mappedBehavior:behavior)
+    //  function mapVulnToPatched(vulnBehaviors:Behavior) : (mappedBehavior:Behavior)
     //     // requires BehaviorEvalsCode(challenge_8_transport_handler_create_conn_vuln(),patchedBehavior)
     //     ensures |vulnBehaviors| == |mappedBehavior|
     //     ensures forall i :: (i >= 0 && i < |vulnBehaviors|) ==> mappedBehavior[i] == patchified(vulnBehaviors[i])
@@ -345,13 +663,13 @@ lemma patchBehavorsTest(s:state,c:seq<Code>) returns (postB:behavior)
         
     // }
 
-    // predicate canMapToVuln(patchedBehavior:behavior)
+    // predicate canMapToVuln(patchedBehavior:Behavior)
     // {
     //     var mappedBehavior := mapPatchedToVuln(patchedBehavior);
     //     BehaviorEvalsCode(challenge_8_transport_handler_create_conn_vuln(),mappedBehavior)
     // }
 
-    // predicate canMapToPatch(vulnBehavior:behavior)
+    // predicate canMapToPatch(vulnBehavior:Behavior)
     // {
     //     var mappedBehavior := mapVulnToPatched(vulnBehavior);
     //     BehaviorEvalsCode(challenge_8_transport_handler_create_conn_patch(),mappedBehavior)
@@ -365,7 +683,7 @@ lemma patchBehavorsTest(s:state,c:seq<Code>) returns (postB:behavior)
 
     // }
 
-    // predicate miniSpec(b:behavior)
+    // predicate miniSpec(b:Behavior)
     // {
     //     true
     // }
@@ -377,7 +695,7 @@ lemma patchBehavorsTest(s:state,c:seq<Code>) returns (postB:behavior)
 
     // }
     
-    // //     predicate completePatch(pre:set<System_s.behavior>,post:set<System_s.behavior>)
+    // //     predicate completePatch(pre:set<System_s.Behavior>,post:set<System_s.Behavior>)
     // // {
     // //     // forall p :: (p in a && !MiniSpec(p)) ==> p in b
 
@@ -394,7 +712,7 @@ lemma patchBehavorsTest(s:state,c:seq<Code>) returns (postB:behavior)
 
     // }
 
-    // // lemma patchIsBenign(s:state,vuln:codeRe,patch:codeRe)
+    // // lemma patchIsBenign(s:State,vuln:codeRe,patch:codeRe)
     // //     requires ValidState(s)
     // //     requires vuln == challenge_8_transport_handler_create_conn_vuln();
     // //     requires patch == challenge_8_transport_handler_create_conn_patch();
